Replace the top-level [IExternal] constructor with a let-binding.

osiris/src/Rocqify.ml
@@ -439,9 +439,6 @@ and structure_item (item : sitem) =
   | IInclude me ->
       c "IInclude" [ mexpr me ]
 
-  | IExternal (x, e) ->
-      c "IExternal" [ var x; expr e ]
-
   | IExtend cs ->
       clist "IExtend" (map var cs)
 
