rocq-osiris/theories/lang/syntax.v
@@ -372,9 +372,6 @@ with sitem :=
   (* An [include] directive [include me]. *)
   | IInclude (me : mexpr)
 
-  (* An external declaration [external x = e]. *)
-  | IExternal (x : var) (e : expr)
-
   (* An extensible variant type extension [type t += cs]. *)
   | IExtend (cs : list name)
 
